theories/Symbolic/Propositions.v
@@ -302,10 +302,9 @@ Module Type SymPropOn
         | angelicv b k => exists v, safe k (env.snoc ι b v)
         | demonicv b k => forall v, safe k (env.snoc ι b v)
         | @assert_vareq _ x σ xIn t msg k =>
-          (let ζ := sub_shift xIn in
-          inst (formula_eq (term_var x) (subst t ζ)) ι /\
           let ι' := env.remove (x∷σ) ι xIn in
-          safe k ι')
+          env.lookup ι xIn = inst t ι' /\
+          safe k ι'
         | @assume_vareq _ x σ xIn t k =>
           let ι' := env.remove (x∷σ) ι xIn in
           env.lookup ι xIn = inst t ι' ->
@@ -389,6 +388,8 @@ Module Type SymPropOn
       induction p; cbn; rewrite ?debug_equiv, ?obligation_equiv; auto;
         try (intuition; fail).
       apply base.exist_proper; eauto.
+      apply Morphisms_Prop.and_iff_morphism; cbn; eauto.
+      now rewrite inst_subst, inst_sub_shift.
     Qed.
 
     (* Lemma safe_persist  {w1 w2 : World} (ω12 : w1 ⊒ w2) *)
@@ -1084,7 +1085,7 @@ Module Type SymPropOn
           exists (env.insert bIn ιe (inst (eq_rect ((Σ1 ▻▻ Σe) - x∷σ) (fun Σ => Term Σ σ) t (Σ1 ▻▻ Σe - x∷σ) (ctx.remove_in_cat_right bIn)) (ι ►► ιe))).
           rewrite safe_assert_msgs_formulas. cbn.
           rewrite env_insert_app, env.remove_insert, env.insert_lookup.
-          rewrite inst_subst, inst_sub_shift, env.remove_insert, ?inst_eq_rect.
+          rewrite ?inst_eq_rect.
           split; auto.
           rewrite map_snd_subst, inst_subst, inst_eq_rect in Hpc.
           now rewrite inst_sub_single2 in Hpc.
@@ -1096,11 +1097,11 @@ Module Type SymPropOn
           rewrite map_snd_subst, inst_subst.
           unfold eq_rect_r. rewrite safe_eq_rect.
           rewrite eq_sym_involutive. split; auto.
-          rewrite inst_subst in Ht.
           rewrite inst_eq_rect.
           rewrite <- env_remove_app.
           rewrite <- inst_sub_shift.
-          now rewrite inst_sub_single_shift.
+          rewrite inst_sub_single_shift; auto.
+          now rewrite inst_sub_shift.
       Qed.
 
       Lemma error_plug_msg {Σ1 Σ2} (ec : ECtx Σ1 Σ2) (msg : EMessage Σ2) :
@@ -1376,5 +1377,357 @@ Module Type SymPropOn
 
   End Postprocessing.
   Import Postprocessing.
+
+  Module Erasure.
+
+    Import SymProp.
+
+    Inductive ETerm : Set :=
+    | eterm_var     (ℓ : 𝑺) (n : nat)
+    | eterm_val     (σ : Ty) (v : Val σ)
+    | eterm_binop   {σ1 σ2 σ3 : Ty} (op : BinOp σ1 σ2 σ3) (t1 : ETerm) (t2 : ETerm)
+    | eterm_neg     (t : ETerm)
+    | eterm_not     (t : ETerm)
+    | eterm_inl     (t : ETerm)
+    | eterm_inr     (t : ETerm)
+    | eterm_union   {U : 𝑼} (K : 𝑼𝑲 U) (t : ETerm)
+    | eterm_record  (R : 𝑹) (ts : NamedEnv (fun _ => ETerm) (𝑹𝑭_Ty R)).
+
+    Inductive EFormula : Type :=
+    | eformula_user (p : 𝑷) (ts : Env (fun _ => ETerm) (𝑷_Ty p))
+    | eformula_bool (t : ETerm)
+    | eformula_prop {Σ' : LCtx} (ζ : Env (fun _ => ETerm) Σ') (P : abstract_named Val Σ' Prop)
+    | eformula_ge (t1 t2 : ETerm)
+    | eformula_gt (t1 t2 : ETerm)
+    | eformula_le (t1 t2 : ETerm)
+    | eformula_lt (t1 t2 : ETerm)
+    | eformula_eq (σ : Ty) (t1 t2 : ETerm)
+    | eformula_neq (σ : Ty) (t1 t2 : ETerm).
+
+    Inductive ESymProp : Type :=
+    | eangelic_binary (o1 o2 : ESymProp)
+    | edemonic_binary (o1 o2 : ESymProp)
+    | eerror
+    | eblock
+    | eassertk (fml : EFormula) (k : ESymProp)
+    | eassumek (fml : EFormula) (k : ESymProp)
+    | eangelicv (b : 𝑺∷Ty) (k : ESymProp)
+    | edemonicv (b : 𝑺∷Ty) (k : ESymProp)
+    | eassert_vareq
+        (x : 𝑺)
+        (σ : Ty)
+        (n : nat)
+        (t : ETerm)
+        (k : ESymProp)
+    | eassume_vareq
+        (x : 𝑺)
+        (σ : Ty)
+        (n : nat)
+        (t : ETerm)
+        (k : ESymProp).
+
+    Definition erase_term {Σ} : forall {σ} (t : Term Σ σ), ETerm :=
+      fix erase {σ} t :=
+        match t with
+        | @term_var _ ℓ _ ℓIn => eterm_var ℓ (ctx.in_at ℓIn)
+        | term_val σ v => eterm_val σ v
+        | term_binop op t1 t2 => eterm_binop op (erase t1) (erase t2)
+        | term_neg t => eterm_neg (erase t)
+        | term_not t => eterm_not (erase t)
+        | term_inl t => eterm_inl (erase t)
+        | term_inr t => eterm_inr (erase t)
+        | term_union U K t => eterm_union K (erase t)
+        | term_record R ts => eterm_record (env.map (fun _ => erase) ts)
+        end.
+
+    Definition erase_formula {Σ} : Formula Σ -> EFormula :=
+      fix erase f :=
+        match f with
+        | formula_user p ts => @eformula_user p (env.map (@erase_term Σ) ts)
+        | formula_bool t => eformula_bool (erase_term t)
+        | formula_prop ζ P =>  eformula_prop (env.map (fun _ => erase_term) ζ) P
+        | formula_ge t1 t2 => eformula_ge (erase_term t1) (erase_term t2)
+        | formula_gt t1 t2 => eformula_gt (erase_term t1) (erase_term t2)
+        | formula_le t1 t2 => eformula_le (erase_term t1) (erase_term t2)
+        | formula_lt t1 t2 => eformula_lt (erase_term t1) (erase_term t2)
+        | @formula_eq _ σ t1 t2 => eformula_eq σ (erase_term t1) (erase_term t2)
+        | @formula_neq _ σ t1 t2 => eformula_neq σ (erase_term t1) (erase_term t2)
+        end.
+
+    Fixpoint erase_symprop {Σ} (p : SymProp Σ) : ESymProp :=
+      match p with
+      | angelic_binary o1 o2 => eangelic_binary (erase_symprop o1) (erase_symprop o2)
+      | demonic_binary o1 o2 => edemonic_binary (erase_symprop o1) (erase_symprop o2)
+      | error _ => eerror
+      | block => eblock
+      | assertk fml _ k => eassertk (erase_formula fml) (erase_symprop k)
+      | assumek fml k => eassumek (erase_formula fml) (erase_symprop k)
+      | angelicv b k => eangelicv b (erase_symprop k)
+      | demonicv b k => edemonicv b (erase_symprop k)
+      | @assert_vareq _ x σ xIn t msg k => eassert_vareq x σ (ctx.in_at xIn) (erase_term t) (erase_symprop k)
+      | @assume_vareq _ x σ xIn t k => eassume_vareq x σ (ctx.in_at xIn) (erase_term t) (erase_symprop k)
+      | debug b k => erase_symprop k
+      end.
+
+    Fixpoint erase_valuation {Σ} (ι : Valuation Σ) : list { σ : Ty & Val σ} :=
+      match ι with
+      | env.nil        => nil
+      | env.snoc ι b v => cons (existT (type b) v) (erase_valuation ι)
+      end.
+
+    Import option.notations.
+
+    Definition inst_namedenv' (ι : list { σ : Ty & Val σ}) (inst_eterm : ETerm -> forall τ, option (Val τ)) {N} :
+      forall {Δ : NCtx N Ty}, NamedEnv (fun _ => ETerm) Δ -> option (NamedEnv Val Δ) :=
+       fix inst_env {Δ} E :=
+         match E with
+         | [] => Some []
+         | @env.snoc _ _ Γ E (ℓ∷σ) t =>
+             v  <- inst_eterm t σ;;
+             vs <- inst_env E;;
+             Some (vs ► (ℓ∷σ ↦ v))
+         end.
+
+    Definition inst_eterm (ι : list { σ : Ty & Val σ}) : ETerm -> forall τ, option (Val τ) :=
+      fix inst_eterm t τ :=
+        match t with
+        | eterm_var _ n =>
+            '(existT σ v) <- nth_error ι n;;
+            match Classes.eq_dec σ τ with
+            | left e => Some (eq_rect σ Val v τ e)
+            | right _ => None
+            end
+        | eterm_val σ v =>
+            match Classes.eq_dec σ τ with
+            | left e => Some (eq_rect σ Val v τ e)
+            | right _ => None
+            end
+        | @eterm_binop σ1 σ2 σ3 op t1 t2 =>
+            match Classes.eq_dec σ3 τ with
+            | left e =>
+                v1 <- inst_eterm t1 σ1;;
+                v2 <- inst_eterm t2 σ2;;
+                Some (eq_rect σ3 Val (eval_binop op v1 v2) τ e)
+            | right _ => None
+            end
+        | eterm_neg t0 =>
+            match Classes.eq_dec ty_int τ with
+            | left e => v <- inst_eterm t0 ty_int;;
+                        Some (eq_rect ty_int Val (BinInt.Z.opp v) τ e)
+            | right _ => None
+            end
+        | eterm_not t0 =>
+            match Classes.eq_dec ty_bool τ with
+            | left e => v <- inst_eterm t0 ty_bool;;
+                        Some (eq_rect ty_bool Val (negb v) τ e)
+            | right _ => None
+            end
+        | eterm_inl t0 =>
+            match τ with
+            | ty_sum τ1 τ2 => v <- inst_eterm t0 τ1 ;; Some (inl v)
+            | _ => None
+            end
+        | eterm_inr t0 =>
+            match τ with
+            | ty_sum τ1 τ2 => v <- inst_eterm t0 τ2 ;; Some (inr v)
+            | _ => None
+            end
+        | @eterm_union U K t0 =>
+            match τ with
+            | ty_union U' =>
+                match Classes.eq_dec U U' with
+                | left e =>
+                    v <- inst_eterm t0 (𝑼𝑲_Ty K);;
+                    Some (eq_rect U 𝑼𝑻 (𝑼_fold (existT K v)) U' e)
+                | right _ => None
+                end
+            | _ => None
+            end
+        | @eterm_record R ts =>
+            match τ with
+            | ty_record R' =>
+                match Classes.eq_dec R R' with
+                | left e =>
+                    v <- inst_namedenv' ι inst_eterm ts;;
+                    Some (eq_rect R 𝑹𝑻 (𝑹_fold v) R' e)
+                | right _ => None
+                end
+            | _ => None
+            end
+        end.
+
+    Definition inst_namedenv (ι : list { σ : Ty & Val σ}) {N} {Δ : NCtx N Ty} :
+      Env (fun _ => ETerm) Δ -> option (NamedEnv Val Δ) :=
+      inst_namedenv' ι (inst_eterm ι).
+
+    Definition inst_env (ι : list { σ : Ty & Val σ}) :
+      forall {Δ : Ctx Ty}, Env (fun _ => ETerm) Δ -> option (Env Val Δ) :=
+      fix inst_env {Δ} E :=
+        match E with
+        | [] => Some []
+        | @env.snoc _ _ Γ E σ t =>
+            v  <- inst_eterm ι t σ;;
+            vs <- inst_env E;;
+            Some (vs ► (σ ↦ v))
+        end.
+
+    Definition inst_eformula (ι : list { σ : Ty & Val σ}) (f : EFormula) : Prop :=
+      match f with
+      | @eformula_user p ts => option_rect (fun _ => Prop) (env.uncurry (𝑷_inst p)) False (inst_env ι ts)
+      | eformula_bool t => option_rect (fun _ => Prop) (fun b => b = true) False (inst_eterm ι t ty_bool)
+      | @eformula_prop Σ' ζ P => option_rect (fun _ => Prop) (uncurry_named P) False (inst_namedenv ι ζ)
+      | eformula_ge t1 t2 => option_rect (fun _ => Prop) (fun '(v1,v2) => BinInt.Z.ge v1 v2) False
+                               (v1 <- inst_eterm ι t1 ty_int;; v2 <- inst_eterm ι t2 ty_int;; Some (v1, v2))
+      | eformula_gt t1 t2 => option_rect (fun _ => Prop) (fun '(v1,v2) => BinInt.Z.gt v1 v2) False
+                               (v1 <- inst_eterm ι t1 ty_int;; v2 <- inst_eterm ι t2 ty_int;; Some (v1, v2))
+      | eformula_le t1 t2 => option_rect (fun _ => Prop) (fun '(v1,v2) => BinInt.Z.le v1 v2) False
+                               (v1 <- inst_eterm ι t1 ty_int;; v2 <- inst_eterm ι t2 ty_int;; Some (v1, v2))
+      | eformula_lt t1 t2 => option_rect (fun _ => Prop) (fun '(v1,v2) => BinInt.Z.lt v1 v2) False
+                               (v1 <- inst_eterm ι t1 ty_int;; v2 <- inst_eterm ι t2 ty_int;; Some (v1, v2))
+      | eformula_eq σ t1 t2 => option_rect (fun _ => Prop) (fun '(v1,v2) => v1 = v2) False
+                                 (v1 <- inst_eterm ι t1 σ;; v2 <- inst_eterm ι t2 σ;; Some (v1, v2))
+      | eformula_neq σ t1 t2 => option_rect (fun _ => Prop) (fun '(v1,v2) => v1 <> v2) False
+                                  (v1 <- inst_eterm ι t1 σ;; v2 <- inst_eterm ι t2 σ;; Some (v1, v2))
+      end.
+
+    Fixpoint list_remove {A} (xs : list A) (n : nat) : list A :=
+      match xs with
+      | nil       => nil
+      | cons x xs => match n with
+                     | O   => xs
+                     | S n => cons x (list_remove xs n)
+                     end
+      end.
+
+    Fixpoint inst_symprop (ι : list { σ : Ty & Val σ}) (f : ESymProp) : Prop :=
+      match f with
+      | eangelic_binary p1 p2 => inst_symprop ι p1 \/ inst_symprop ι p2
+      | edemonic_binary p1 p2 => inst_symprop ι p1 /\ inst_symprop ι p2
+      | eerror => False
+      | eblock => True
+      | eassertk fml k => inst_eformula ι fml /\ inst_symprop ι k
+      | eassumek fml k => inst_eformula ι fml -> inst_symprop ι k
+      | eangelicv b k => exists v : Val (type b), inst_symprop (cons (existT (type b) v) ι) k
+      | edemonicv b k => forall v : Val (type b), inst_symprop (cons (existT (type b) v) ι) k
+      | eassert_vareq x σ n t k =>
+          let ι' := list_remove ι n in
+          inst_eterm ι (eterm_var x n) σ = inst_eterm ι' t σ /\
+          inst_symprop ι' k
+      | eassume_vareq x σ n t k =>
+          let ι' := list_remove ι n in
+          inst_eterm ι (eterm_var x n) σ = inst_eterm ι' t σ ->
+          inst_symprop ι' k
+      end.
+
+    Lemma erase_valuation_remove {Σ b} (bIn : b ∈ Σ) (ι : Valuation Σ) :
+      list_remove (erase_valuation ι) (ctx.in_at bIn) =
+      erase_valuation (env.remove b ι bIn).
+    Proof.
+      induction ι.
+      - destruct (ctx.nilView bIn).
+      - destruct (ctx.snocView bIn); cbn.
+        + reflexivity.
+        + f_equal. apply (IHι i).
+    Qed.
+
+    Lemma nth_error_erase {Σ b} (ι : Valuation Σ) (bIn : b ∈ Σ) :
+      nth_error (erase_valuation ι) (ctx.in_at bIn) =
+      Some (existT (type b) (env.lookup ι bIn)).
+    Proof.
+      induction ι; cbn.
+      - destruct (ctx.nilView bIn).
+      - destruct (ctx.snocView bIn) as [|b bIn]; cbn.
+        + reflexivity.
+        + now rewrite IHι.
+    Qed.
+
+    Lemma inst_eterm_erase {Σ σ} (t : Term Σ σ) (ι : Valuation Σ) :
+      inst_eterm (erase_valuation ι) (erase_term t) σ = Some (inst t ι).
+    Proof.
+      induction t; cbn [inst_eterm erase_term].
+      - rewrite nth_error_erase; cbn.
+        now rewrite EqDec.eq_dec_refl.
+      - now rewrite EqDec.eq_dec_refl.
+      - now rewrite EqDec.eq_dec_refl, IHt1, IHt2.
+      - now rewrite IHt.
+      - now rewrite IHt.
+      - now rewrite IHt.
+      - now rewrite IHt.
+      - now rewrite EqDec.eq_dec_refl, IHt.
+      - rewrite EqDec.eq_dec_refl. cbn.
+        assert (inst_namedenv'
+                  (erase_valuation ι)
+                  (inst_eterm (erase_valuation ι))
+                  (env.map (fun b : 𝑹𝑭∷Ty => erase_term) es) =
+                  Some (inst
+                    (* (T := fun Σ => @NamedEnv 𝑹𝑭 Ty (Term Σ) (𝑹𝑭_Ty R)) *)
+                    (* (A := @NamedEnv 𝑹𝑭 Ty Val (𝑹𝑭_Ty R)) *)
+                    es ι)) as ->; auto.
+        induction IH as [|Δ E [x σ] t _ IHE IHt]; cbn in *.
+        + reflexivity.
+        + now rewrite IHt, IHE.
+    Qed.
+
+    Lemma inst_env_erase {Σ Δ} (ts : Env (Term Σ) Δ) (ι : Valuation Σ) :
+      inst_env (erase_valuation ι) (env.map (@erase_term Σ) ts) = Some (inst ts ι).
+    Proof.
+      induction ts; cbn.
+      - reflexivity.
+      - now rewrite inst_eterm_erase, IHts.
+    Qed.
+
+    Lemma inst_namedenv_erase {Σ N} {Δ : NCtx N Ty} (ts : NamedEnv (Term Σ) Δ) (ι : Valuation Σ) :
+      inst_namedenv (erase_valuation ι) (env.map (fun _ => erase_term) ts) = Some (inst ts ι).
+    Proof.
+      unfold inst_namedenv.
+      induction ts as [|Δ ts IHts [x σ]]; cbn.
+      - reflexivity.
+      - now rewrite inst_eterm_erase, IHts.
+    Qed.
+
+    Lemma inst_eformula_erase {Σ} (fml : Formula Σ) (ι : Valuation Σ) :
+      inst_eformula (erase_valuation ι) (erase_formula fml) <-> inst fml ι.
+    Proof.
+      destruct fml; cbn;
+        now rewrite ?inst_eterm_erase, ?inst_env_erase, ?inst_namedenv_erase.
+    Qed.
+
+    Lemma erase_safe {Σ} (p : 𝕊 Σ) (ι : Valuation Σ) :
+      inst_symprop (erase_valuation ι) (erase_symprop p) <->
+      safe p ι.
+    Proof.
+      induction p; cbn [inst_symprop erase_symprop safe].
+      - apply Morphisms_Prop.or_iff_morphism. auto. auto.
+      - apply Morphisms_Prop.and_iff_morphism. auto. auto.
+      - reflexivity.
+      - reflexivity.
+      - apply Morphisms_Prop.and_iff_morphism.
+        + apply inst_eformula_erase.
+        + auto.
+      - apply Morphisms_Prop.iff_iff_iff_impl_morphism.
+        + apply inst_eformula_erase.
+        + auto.
+      - apply base.exist_proper. intros v. apply (IHp (env.snoc ι b v)).
+      - apply base.forall_proper. intros v. apply (IHp (env.snoc ι b v)).
+      - apply Morphisms_Prop.and_iff_morphism; cbn.
+        + rewrite nth_error_erase; cbn.
+          rewrite EqDec.eq_dec_refl.
+          rewrite erase_valuation_remove. cbn.
+          rewrite inst_eterm_erase.
+          intuition.
+        + generalize (IHp (env.remove _ ι xIn)).
+          now rewrite erase_valuation_remove.
+      - apply Morphisms_Prop.iff_iff_iff_impl_morphism; cbn.
+        + rewrite nth_error_erase; cbn.
+          rewrite EqDec.eq_dec_refl.
+          rewrite erase_valuation_remove. cbn.
+          rewrite inst_eterm_erase.
+          intuition.
+        + generalize (IHp (env.remove _ ι xIn)).
+          now rewrite erase_valuation_remove.
+      - apply IHp.
+    Qed.
+
+  End Erasure.
 
 End SymPropOn.
